x86/Asmexpand.ml
@@ -480,8 +480,7 @@ let set_al sg =
 
 let expand_instruction instr =
   match instr with
-  | Pallocframe (f, ofs_ra) ->
-let sz = StackADT.frame_size f in
+  |  Pallocframe (sz, _, ofs_ra) ->
      if Archi.ptr64 then begin
        let (sz, save_regs) = sp_adjustment_64 sz in
        (* Allocate frame *)
